WIP on LinkedJournal

Splinter/Journal/LinkedJournal.i.dfy
@@ -2,6 +2,7 @@
 // SPDX-License-Identifier: BSD-2-Clause
 
 include "../CoordinationLayer/AbstractJournal.i.dfy"
+include "PagedJournal.i.dfy"
 
 module LinkedJournal {
   import opened Options
@@ -10,132 +11,30 @@ module LinkedJournal {
   import opened Sequences
   import PagedJournal
 
-  datatype CacheView = CacheView(entries: map<Pointer, JournalRecord>) {
-    function I(boundaryLSN: LSN, pointer: Pointer, used: set<Pointer>) : Option<PagedJournal.JournalRecord>
-      decreases entries.Keys - used, 0
-    {
-      if pointer in used
-      then None // Pointer cycle; fail.
-      else if pointer !in entries
-      then None
-      else
-        Some(entries[pointer].CacheI(boundaryLSN, this, used + {pointer}))
-    }
+  type Address(!new, ==)
+  type Pointer = Option<Address>
+
+  // TODO(robj): where does this go?
+  datatype DiskView = DiskView(entries: map<Address, JournalRecord>) {
   }
 
-  datatype JournalRecord = JournalRecord(
-    messageSeq: MsgHistory,
-    priorRec: Option<Pointer>
-  )
+  datatype JournalRecord = JournalRecord(messageSeq: MsgHistory, priorRec: Pointer)
   {
     predicate WF()
     {
       messageSeq.WF()
     }
-    
-    function CacheI(boundaryLSN: LSN, cacheView: CacheView, used: set<Pointer>) : PagedJournal.JournalRecord
-      decreases cacheView.entries.Keys - used, 1
-    {
-      PagedJournal.JournalRecord(messageSeq,
-        if messageSeq.seqStart <= boundaryLSN
-        then None // no need to advance
-        else if priorRec.None?
-        then None // nowhere to go
-        else cacheView.I(boundaryLSN, priorRec.value, used))
-    }
   }
-
+    
   datatype TruncatedJournal = TruncatedJournal(
     boundaryLSN : LSN,  // exclusive: lsns <= boundaryLSN are discarded
-    freshestRec: Option<Pointer>,
-    cacheView: CacheView)
-  {
-    function I() : PagedJournal.TruncatedJournal
-    {
-      PagedJournal.TruncatedJournal(boundaryLSN,
-        if freshestRec.None? then None
-        else cacheView.I(boundaryLSN, freshestRec.value, {}))
-    }
-
-    predicate WF()
-    {
-      I()..BuildReceiptTJ().TJValid()
-    }
-  }
+    freshestRec: Pointer,
+    cacheView: DiskView)
 
   function Mkfs() : (out:TruncatedJournal)
   {
-    // TODO(jonh): Just making up CacheViews seems like trouble for lower in the stack.
-    TruncatedJournal(0, None, CacheView(map[]))
-  }
-
-  lemma DiscardOldLemma(cacheView: CacheView, oldBoundary: LSN, newBoundary: LSN, pointer: Pointer, used: set<Pointer>)
-    requires cacheView.I(oldBoundary, pointer, used).Some?
-    requires TruncatedJournal(oldBoundary, cacheView.I(oldBoundary, pointer, used)).WF()
-    requires TruncatedJournal(oldBoundary, cacheView.I(oldBoundary, pointer, used)).I().CanDiscardTo(newBoundary)
-    ensures TruncatedJournal(oldBoundary, cacheView.I(oldBoundary, pointer, used)).DiscardOld(newBoundary)
-      == TruncatedJournal(newBoundary, cacheView.I(newBoundary, pointer, used))
-  {
-    if pointer in used {
-      // Pointer cycle; fail.
-      assert TruncatedJournal(oldBoundary, cacheView.I(oldBoundary, pointer, used)).DiscardOld(newBoundary)
-        == TruncatedJournal(newBoundary, cacheView.I(newBoundary, pointer, used));
-    } else if pointer !in cacheView.entries {
-      assert TruncatedJournal(oldBoundary, cacheView.I(oldBoundary, pointer, used)).DiscardOld(newBoundary)
-        == TruncatedJournal(newBoundary, cacheView.I(newBoundary, pointer, used));
-    } else {
-      var entry := cacheView.entries[pointer];
-      if entry.messageSeq.seqStart <= oldBoundary {
-        /*
-        Wait we've already done all this reasoning before.
-        *All* we should be doing right now is showing a connection between the
-        linked representation and the nested representation.
-        The only time they might diverge is if there's a cycle or missing link,
-        but those should look exactly like a None.
-        So what I really want is a lemma that says:
-
-        cacheView.I(x, pointer, used) == cacheView.I(y, pointer, used)
-
-        hmm, does the CacheView change if the boundary changes?
-        What happens in the nested view? Do we stop nesting? No, or yes -- they
-        should have the same interpretation.
-
-        Yeah, at the nested level we buildReceipt, then DiscardOld.
-        So maybe we shouldn't have plumbed boundaries through the interp!
-
-        So we'd like to argue that
-        buildReceipt(cacheView.I(pointer, used)) == buildReceipt(cacheView.I(pointer, used))
-
-        (1) 
-        [10 o 20][20 n 30][30   40]
-
-        [10 o 20][20 n 30][30   40]
-        */
-        // Need to think here
-        calc {
-          cacheView.I(oldBoundary, pointer, used);
-          entry.CacheI(oldBoundary, cacheView, used + {pointer});
-          Some(JournalRecord(entry.messageSeq, None));
-        }
-        calc {
-          cacheView.I(newBoundary, pointer, used);
-          entry.CacheI(oldBoundary, cacheView, used + {pointer});
-          Some(JournalRecord(entry.messageSeq, None));
-        }
-        assert TruncatedJournal(oldBoundary, cacheView.I(oldBoundary, pointer, used)).freshestRec
-          == Some(JournalRecord(entry.messageSeq, None));
-        assert TruncatedJournal(oldBoundary, cacheView.I(oldBoundary, pointer, used)).DiscardOld(newBoundary)
-          == TruncatedJournal(newBoundary, cacheView.I(newBoundary, pointer, used));
-      } else if entry.priorRec.None? {
-        assert TruncatedJournal(oldBoundary, cacheView.I(oldBoundary, pointer, used)).DiscardOld(newBoundary)
-          == TruncatedJournal(newBoundary, cacheView.I(newBoundary, pointer, used));
-      } else {
-        // Need a recursive call here
-        assume false;
-        assert TruncatedJournal(oldBoundary, cacheView.I(oldBoundary, pointer, used)).DiscardOld(newBoundary)
-        == TruncatedJournal(newBoundary, cacheView.I(newBoundary, pointer, used));
-      }
-    }
+    // TODO(jonh): Just making up DiskViews seems like trouble for lower in the stack.
+    TruncatedJournal(0, None, DiskView(map[]))
   }
 
   datatype Variables = Variables(
@@ -146,9 +45,7 @@ module LinkedJournal {
     predicate WF() {
       && truncatedJournal.WF()
       && unmarshalledTail.WF()
-      && (unmarshalledTail.MsgHistory? ==>
-          truncatedJournal.I().CanConcat(unmarshalledTail)
-         )
+      && truncatedJournal.SeqEnd() == unmarshalledTail.seqStart
     }
   }
 
@@ -191,46 +88,22 @@ module LinkedJournal {
   }
 
   datatype Step =
-      PutStep(msgs: MsgHistory)
+      ReadForRecoveryStep(receiptIndex: nat)
+    | FreezeForCommitStep(keepReceiptLines: nat)
+    | ObserveFreshJournalLabel()
+    | PutStep(msgs: MsgHistory)
     | DiscardOldStep(lsn: LSN)
-    | JournalMarshalStep(cut: LSN)
+    | InternalJournalMarshalStep(cut: LSN)
 
   predicate NextStep(v: Variables, v': Variables, step: Step)
   {
     match step {
-      case PutStep(msgs) => Put(v, v', msgs)
-      case DiscardOldStep(lsn) => DiscardOld(v, v', lsn)
-      case JournalMarshalStep(cut) => JournalMarshal(v, v', cut)
+      case ReadForRecoveryStep(receiptIndex) => ReadForRecovery(v, v', lbl, receiptIndex)
+      case FreezeForCommitStep(keepReceiptLines) => FreezeForCommit(v, v', lbl, keepReceiptLines)
+      case ObserveFreshJournalLabel() => ObserveFreshJournal(v, v', lbl)
+      case PutStep() => Put(v, v', lbl)
+      case DiscardOldStep() => DiscardOld(v, v', lbl)
+      case InternalJournalMarshalStep(cut) => InternalJournalMarshal(v, v', lbl, cut)
     }
   }
-
-  function TJ_DiscardOld(self: TruncatedJournalType, lsn: LSN) : (out:TruncatedJournalType)
-    //requires TJ_WF(self)
-    //requires TJ_I(self).I().CanDiscardTo(lsn)
-    //ensures TJ_WF(out)
-    //ensures TJ_I(out) == TJ_I(self).DiscardOld(lsn)
-  {
-    var out := TruncatedJournalType(lsn, self.freshestRec, self.cacheView);
-    assert out.I() == self.I().DiscardOld(lsn);
-    assert TJ_WF(out);
-    assert TJ_I(out) == TJ_I(self).DiscardOld(lsn);
-    out
-  }
-
-  function TJ_DiscardRecent(self: TruncatedJournalType, i: nat) : (out:TruncatedJournalType)
-    //requires TJ_WF(self)
-    //requires TJ_CanDiscardRecentAtLine(self, i)
-    //ensures TJ_WF(out)
-    //ensures
-    //  var receipt := TJ_I(self).BuildReceiptTJ();
-    //  TJ_I(out) == TruncatedJournal(TJ_I(self).boundaryLSN, Some(receipt.lines[i].journalRec))
-
-  function TJ_AppendRecord(self: TruncatedJournalType, msgs: MsgHistory) : (out:TruncatedJournalType)
-    //requires TJ_WF(self)
-    //requires msgs.MsgHistory?
-    //requires TJ_I(self).Empty() || msgs.CanFollow(TJ_I(self).SeqEnd())
-    //ensures TJ_WF(out)
-    //ensures TJ_I(out) == TruncatedJournal(
-    //  TJ_AppendNewBoundary(self, msgs),
-    //  Some(JournalRecord(msgs, TJ_I(self).freshestRec)))
 }
